start updating compile_val to allow global env to change
the old statement made no mention of the globals field of the bytecode
state (since it didn't exist), but we have to say something about it for
the compilation of extend/init gvar. i am hoping the relation i've
defined saying the global env grows monotonically is sufficient.

compiler/proofs/bytecodeProofScript.sml
@@ -401,12 +401,18 @@ val lookup_ct_imp_incsz_many = store_thm("lookup_ct_imp_incsz_many",
   fsrw_tac[ARITH_ss][])
 
 val lookup_ct_change_refs = store_thm("lookup_ct_change_refs",
-  ``∀sz st rf rf' gv ct.
+  ``∀sz st rf rf' gv gv' ct.
     (∀n vs p. (ct = CTEnv (CCRef n)) ∧ sz < LENGTH st ∧ (EL sz st = Block 0 vs) ∧ n < LENGTH vs ∧ (EL n vs = RefPtr p) ⇒
-       (FLOOKUP rf' p = FLOOKUP rf p))
-    ⇒ (lookup_ct sz st rf' gv ct = lookup_ct sz st rf gv ct)``,
+       (FLOOKUP rf' p = FLOOKUP rf p)) ∧
+    (*
+    LENGTH gv ≤ LENGTH gv' ∧
+    (∀n. LENGTH gv ≤ n ∧ n < LENGTH gv' ⇒ EL n gv' = NONE) ∧
+    *)
+    (∀n. (ct = CTDec n) ⇒ n < LENGTH gv ∧ n < LENGTH gv' ∧ EL n gv' = EL n gv)
+    ⇒ (lookup_ct sz st rf' gv' ct = lookup_ct sz st rf gv ct)``,
   rw[LET_THM] >>
-  Cases_on`ct`>>fs[] >> rw[] >>
+  Cases_on`ct`>>fs[] >> rw[el_check_def] >> fs[] >>
+  fsrw_tac[ARITH_ss][] >>
   Cases_on`c`>>fs[el_check_def]>>
   Cases_on`EL sz st`>>fs[] >> rw[]>>fs[]>>
   BasicProvers.CASE_TAC>>fs[]>>
@@ -599,9 +605,8 @@ val Cenv_bs_CTLet_bound = store_thm("Cenv_bs_CTLet_bound",
   match_mp_tac (GEN_ALL env_renv_CTLet_bound) >>
   metis_tac[])
 
-(*
 val env_renv_CTDec_bound = store_thm("env_renv_CTDec_bound",
-  ``env_renv rd rsz bs env renv ∧ CTDec n ∈ set renv ⇒ n < LENGTH bs.stack``,
+  ``env_renv rd rsz bs env renv ∧ CTDec n ∈ set renv ⇒ n < LENGTH bs.globals``,
   rw[EVERY2_EVERY,EVERY_MEM,FORALL_PROD,env_renv_def] >>
   rfs[MEM_ZIP,MEM_EL] >> fsrw_tac[DNF_ss][] >>
   qmatch_assum_abbrev_tac `z < LENGTH E`>>
@@ -611,11 +616,16 @@ val env_renv_CTDec_bound = store_thm("env_renv_CTDec_bound",
   srw_tac[ARITH_ss][])
 
 val Cenv_bs_CTDec_bound = store_thm("Cenv_bs_CTDec_bound",
-  ``Cenv_bs rd menv s env rmenv renv rsz csz bs ∧ (CTDec n) ∈ set renv ⇒ n < LENGTH bs.stack``,
-  rw[Cenv_bs_def,fmap_rel_def,IN_FRANGE] >>
+  ``Cenv_bs rd s env renv rsz csz bs ∧ (CTDec n) ∈ set renv ⇒ n < LENGTH bs.globals``,
+  rw[Cenv_bs_def] >>
   match_mp_tac (GEN_ALL env_renv_CTDec_bound) >>
   metis_tac[])
 
+val CTDec_bound_lemma =
+  CONJ (prove(``∀x y. (x with code := y).stack = x.stack``,simp[]))
+       (SIMP_RULE(srw_ss())[]Cenv_bs_CTDec_bound)
+
+(*
 val env_renv_imp_incsz_CTDec = store_thm("env_renv_imp_incsz_CTDec",
   ``∀rd sz bs menv cmnv bs' vs.
     env_renv rd sz bs menv (MAP CTDec cmnv) ∧ (bs' = bs with stack := vs ++ bs.stack) ⇒
@@ -638,10 +648,6 @@ val fmap_rel_env_renv_CTDec = store_thm("fmap_rel_env_renv_CTDec",
    qexists_tac`bs` >>
    simp[bc_state_component_equality] >>
    metis_tac[o_f_FAPPLY])
-
-val CTDec_bound_lemma =
-  CONJ (prove(``∀x y. (x with code := y).stack = x.stack``,simp[]))
-       (SIMP_RULE(srw_ss())[]Cenv_bs_CTDec_bound)
 *)
 
 val Cenv_bs_pops = store_thm("Cenv_bs_pops",
@@ -803,12 +809,24 @@ val Cenv_bs_DOMSUB = store_thm("Cenv_bs_DOMSUB",
   rw[Cenv_bs_def,EVERY2_EVERY,env_renv_def,fmap_rel_def] >>
   metis_tac[o_f_FAPPLY])
 
+val gvrel_def = Define`
+  gvrel gv1 gv2 ⇔ LENGTH gv1 ≤ LENGTH gv2 ∧
+    (∀n x. n < LENGTH gv1 ∧ (EL n gv1 = SOME x) ⇒ (EL n gv2 = SOME x))`
+
+val gvrel_refl = store_thm("gvrel_refl",
+  ``gvrel g g``, rw[gvrel_def])
+val _ = export_rewrites["gvrel_refl"]
+
+val gvrel_trans = store_thm("gvrel_trans",
+  ``gvrel gv1 gv2 ∧ gvrel gv2 gv3 ⇒ gvrel gv1 gv3``,
+  rw[gvrel_def] >> fsrw_tac[ARITH_ss][])
+
 val env_renv_change_store = store_thm("env_renv_change_store",
   ``env_renv rd rsz bs env renv ∧
-    (bs' = bs with <| refs := rfs'; clock := ck'|>) ∧
+    (bs' = bs with <| refs := rfs'; clock := ck'; globals := gv'|>) ∧
     s_refs rd s bs ∧
-    s_refs rd' s' (bs with <|refs := rfs'; clock := ck'|>) ∧
-    rd.sm ≼ rd'.sm ∧ rd.cls ⊑ rd'.cls ∧
+    s_refs rd' s' bs' ∧
+    rd.sm ≼ rd'.sm ∧ rd.cls ⊑ rd'.cls ∧ gvrel bs.globals gv' ∧
     DRESTRICT bs.refs (COMPL (set rd.sm)) ⊑ DRESTRICT rfs' (COMPL (set rd'.sm))
     ⇒
     env_renv rd' rsz bs' env renv``,
@@ -819,10 +837,17 @@ val env_renv_change_store = store_thm("env_renv_change_store",
   `X = X'` by (
     unabbrev_all_tac >>
     match_mp_tac lookup_ct_change_refs >>
+    conj_tac >- (
+      rpt gen_tac >> strip_tac >>
+      fs[s_refs_def,good_rd_def,FEVERY_DEF,UNCURRY,el_check_def] >>
+      fs[SUBMAP_DEF,FDOM_DRESTRICT,FLOOKUP_DEF,DRESTRICT_DEF] >>
+      metis_tac[] ) >>
     rpt gen_tac >> strip_tac >>
-    fs[s_refs_def,good_rd_def,FEVERY_DEF,UNCURRY,el_check_def] >>
-    fs[SUBMAP_DEF,FDOM_DRESTRICT,FLOOKUP_DEF,DRESTRICT_DEF] >>
-    metis_tac[] ) >>
+    rfs[s_refs_def,EVERY2_EVERY,gvrel_def] >>
+    fs[option_case_NONE_F] >> res_tac >>
+    fs[el_check_def] >>
+    BasicProvers.EVERY_CASE_TAC >> fs[] >>
+    fsrw_tac[ARITH_ss][] ) >>
   simp[Abbr`Z`] >>
   match_mp_tac (MP_CANON (GEN_ALL (CONJUNCT1 (SPEC_ALL Cv_bv_SUBMAP)))) >>
   HINT_EXISTS_TAC >>
@@ -831,16 +856,17 @@ val env_renv_change_store = store_thm("env_renv_change_store",
   fs[SUBMAP_DEF,SUBSET_DEF,DRESTRICT_DEF,IN_FRANGE] )
 
 val Cenv_bs_change_store = store_thm("Cenv_bs_change_store",
-  ``∀rd s env renv rsz csz bs rd' s' bs' rfs' ck'.
+  ``∀rd s env renv rsz csz bs rd' s' bs' rfs' ck' gv'.
     Cenv_bs rd s env renv rsz csz bs ∧
     s_refs rd' s' bs' ∧
-    (bs' = bs with <| refs := rfs'; clock := ck' |>) ∧
+    (bs' = bs with <| refs := rfs'; clock := ck'; globals := gv' |>) ∧
     DRESTRICT bs.refs (COMPL (set rd.sm)) ⊑ DRESTRICT rfs' (COMPL (set rd'.sm)) ∧
-    rd.sm ≼ rd'.sm ∧ rd.cls ⊑ rd'.cls
+    rd.sm ≼ rd'.sm ∧ rd.cls ⊑ rd'.cls ∧ gvrel bs.globals gv'
     ⇒
     Cenv_bs rd' s' env renv rsz csz bs'``,
   rw[Cenv_bs_def,EVERY2_EVERY,EVERY_MEM,FORALL_PROD,fmap_rel_def] >>
   match_mp_tac (GEN_ALL env_renv_change_store) >>
+  first_assum (match_exists_tac o concl) >> simp[] >>
   metis_tac[])
 
 val Cenv_bs_perm = store_thm("Cenv_bs_perm",
@@ -1232,6 +1258,7 @@ val prim1_to_bc_thm = store_thm("prim1_to_bc_thm",
       Cv_bv (mk_pp rd' (bs' with <| code := bce |>)) v bv ∧
       s_refs rd' ((ck,FST s'),SND s') (bs' with code := bce) ∧
       DRESTRICT bs.refs (COMPL (set rd.sm)) ⊑ DRESTRICT rf (COMPL (set sm')) ∧
+      gvrel bs.globals gv ∧
       rd.sm ≼ sm'``,
   simp[] >> rw[] >>
   `bc_fetch bs = SOME (HD (prim1_to_bc op))` by (
@@ -1361,8 +1388,10 @@ val prim1_to_bc_thm = store_thm("prim1_to_bc_thm",
     fs[s_refs_def,good_rd_def] >>
     rfs[EVERY2_EVERY,EVERY_MEM] >>
     fs[MEM_ZIP,PULL_EXISTS] >>
-    simp[EL_LUPDATE] >> rw[] >>
-    rw[optionTheory.OPTREL_def]))
+    simp[gvrel_def,EL_LUPDATE] >> rw[] >>
+    rw[optionTheory.OPTREL_def] >>
+    fs[optionTheory.OPTREL_def] >>
+    metis_tac[optionTheory.NOT_SOME_NONE]))
 
 (* compile_closures *)
 
@@ -2009,6 +2038,10 @@ val compile_closures_thm = store_thm("compile_closures_thm",
       lrw[Abbr`ls`,LIST_EQ_REWRITE,EL_DROP,EL_APPEND2] ) >>
     simp[] >>
     match_mp_tac lookup_ct_change_refs >>
+    reverse conj_tac >- (
+      rw[] >>
+      ntac 2 (first_x_assum(qspec_then`n`mp_tac)) >>
+      simp[el_check_def] >> rw[] ) >>
     rw[] >>
     simp[FLOOKUP_DEF,FDOM_FUPDATE_LIST,MEM_MAP,EXISTS_PROD,DRESTRICT_DEF] >>
     `¬MEM p rs` by (
@@ -2069,6 +2102,12 @@ val compile_closures_thm = store_thm("compile_closures_thm",
     simp[Abbr`ls`,DROP_APPEND2] >>
     AP_TERM_TAC >>
     match_mp_tac lookup_ct_change_refs >>
+    reverse conj_tac >- (
+      rw[] >>
+      fs[EVERY_MEM] >>
+      res_tac >> fs[UNCURRY] >>
+      ntac 2 (first_x_assum(qspec_then`n`mp_tac)) >>
+      simp[el_check_def] >> rw[] ) >>
     simp[] >> rw[] >> fs[FLOOKUP_DEF] >>
     simp[DRESTRICT_DEF,FDOM_FUPDATE_LIST,MEM_MAP,EXISTS_PROD] >>
     `¬MEM p rs` by (
@@ -2637,23 +2676,24 @@ val jmpbc_thm = store_thm("jmpbc_thm",
 
 val code_for_push_def = Define`
   code_for_push rd bs bce bc0 code s' env vs renv rsz csz =
-    ∃bvs rf rd' ck.
-    let bs' = bs with <| stack := (REVERSE bvs)++bs.stack; pc := next_addr bs.inst_length (bc0 ++ code); refs := rf; clock := ck |> in
+    ∃bvs rf rd' ck gv.
+    let bs' = bs with <| stack := (REVERSE bvs)++bs.stack; pc := next_addr bs.inst_length (bc0 ++ code);
+                         refs := rf; clock := ck; globals := gv |> in
     bc_next^* bs bs' ∧
     EVERY2 (Cv_bv (mk_pp rd' (bs' with code := bce))) vs bvs ∧
     Cenv_bs rd' s' env renv (rsz+(LENGTH vs)) csz (bs' with code := bce) ∧
     DRESTRICT bs.refs (COMPL (set rd.sm)) ⊑ DRESTRICT rf (COMPL (set rd'.sm)) ∧
-    rd.sm ≼ rd'.sm ∧ rd.cls ⊑ rd'.cls`
+    rd.sm ≼ rd'.sm ∧ rd.cls ⊑ rd'.cls ∧ gvrel bs.globals gv`
 
 val code_for_return_def = Define`
   code_for_return rd bs bce st ret sp v s' =
-    ∃bv rf rd' ck.
-    let bs' = bs with <| stack := bv::st; pc := ret; refs := rf; clock := ck; handler := sp |> in
+    ∃bv rf rd' ck gv.
+    let bs' = bs with <| stack := bv::st; pc := ret; refs := rf; clock := ck; handler := sp; globals := gv |> in
     bc_next^* bs bs' ∧
     Cv_bv (mk_pp rd' (bs' with code := bce)) v bv ∧
     s_refs rd' s' (bs' with code := bce) ∧
     DRESTRICT bs.refs (COMPL (set rd.sm)) ⊑ DRESTRICT rf (COMPL (set rd'.sm)) ∧
-    rd.sm ≼ rd'.sm ∧ rd.cls ⊑ rd'.cls`
+    rd.sm ≼ rd'.sm ∧ rd.cls ⊑ rd'.cls ∧ gvrel bs.globals gv`
 
 val code_for_push_return = store_thm("code_for_push_return",
   ``∀rd bs bce bc0 code s' env v renv rsz csz bc1 args args1 bs' blvs benv st cl cl1 ret hdl.
@@ -2665,7 +2705,7 @@ val code_for_push_return = store_thm("code_for_push_return",
     code_for_return rd bs bce st ret hdl v s'``,
     rw[code_for_push_def,code_for_return_def,LET_THM] >>
     qmatch_assum_rename_tac `Cv_bv pp v bv`["pp"] >>
-    map_every qexists_tac [`bv`,`rf`,`rd'`,`ck`] >>
+    map_every qexists_tac [`bv`,`rf`,`rd'`,`ck`,`gv`] >>
     fs[Cenv_bs_def,s_refs_def,good_rd_def] >>
     qmatch_assum_abbrev_tac`bc_next^* bs0 bs1` >>
     rw[] >>
@@ -2687,7 +2727,7 @@ val code_for_return_append_code = store_thm("code_for_return_append_code",
     code_for_return rd bs' bce st hdl sp v s'``,
   simp[code_for_return_def] >>
   rpt gen_tac >> strip_tac >>
-  map_every qexists_tac[`bv`,`rf`,`rd'`,`ck`] >> fs[] >>
+  map_every qexists_tac[`bv`,`rf`,`rd'`,`ck`,`gv`] >> fs[] >>
   match_mp_tac RTC_bc_next_append_code >>
   qexists_tac`bs` >>
   HINT_EXISTS_TAC >>
@@ -2937,8 +2977,8 @@ fun tac18 t =
     disch_then (mp_tac o CONJUNCT1) >>
     simp[code_for_push_def,code_for_return_def] >>
     simp_tac(srw_ss()++DNF_ss)[] >>
-    map_every qx_gen_tac[`rf`,`rd'`,`ck`,`ev`] >> strip_tac >>
-    map_every qexists_tac[`ev`,`rf`,`rd'`,`ck`] >>
+    map_every qx_gen_tac[`rf`,`rd'`,`ck`,`gv`,`ev`] >> strip_tac >>
+    map_every qexists_tac[`ev`,`rf`,`rd'`,`ck`,`gv`] >>
     conj_tac >- (
       qmatch_assum_abbrev_tac`bc_next^* bs bs2` >>
       match_mp_tac(SIMP_RULE std_ss [transitive_def] RTC_TRANSITIVE) >>
@@ -3049,9 +3089,9 @@ fun tac18 t =
       simp[Abbr`bss0`,TAKE_APPEND1,TAKE_APPEND2] >>
       simp[code_for_push_def] >>
       simp_tac(srw_ss()++DNF_ss)[] >>
-      map_every qx_gen_tac[`rf`,`rd'`,`ck`,`bv`] >>
+      map_every qx_gen_tac[`rf`,`rd'`,`ck`,`gv`,`bv`] >>
       strip_tac >>
-      map_every qexists_tac[`rf`,`rd'`,`ck`,`bv`] >>
+      map_every qexists_tac[`rf`,`rd'`,`ck`,`gv`,`bv`] >>
       conj_tac >- (
         qmatch_assum_abbrev_tac`bc_next^* bs2 bs3` >>
         qmatch_abbrev_tac`bc_next^* bs bs5` >>
@@ -3183,9 +3223,9 @@ fun tac18 t =
     simp[Abbr`bss0`,TAKE_APPEND1,TAKE_APPEND2] >>
     simp[code_for_push_def,code_for_return_def] >>
     simp_tac(srw_ss()++DNF_ss)[] >>
-    map_every qx_gen_tac[`rf`,`rd'`,`ck`,`bv`] >>
+    map_every qx_gen_tac[`rf`,`rd'`,`ck`,`gvv`,`bv`] >>
     strip_tac >>
-    map_every qexists_tac[`bv`,`rf`,`rd'`,`ck`] >>
+    map_every qexists_tac[`bv`,`rf`,`rd'`,`ck`,`gvv`] >>
     conj_tac >- (
       qmatch_assum_abbrev_tac`bc_next^* bs2 bs3` >>
       qmatch_abbrev_tac`bc_next^* bss bs5` >>
@@ -3425,9 +3465,9 @@ fun tac18 t =
       disch_then(mp_tac o CONJUNCT1) >>
       simp[code_for_push_def] >>
       simp_tac(srw_ss()++DNF_ss)[] >>
-      map_every qx_gen_tac[`rf'`,`rd''`,`ck'`,`br`] >>
+      map_every qx_gen_tac[`rf'`,`rd''`,`ck'`,`gvv`,`br`] >>
       strip_tac >>
-      map_every qexists_tac[`rf'`,`rd''`,`ck'`,`br`] >>
+      map_every qexists_tac[`rf'`,`rd''`,`ck'`,`gvv`,`br`] >>
       conj_tac >- (
         match_mp_tac(SIMP_RULE std_ss [transitive_def] RTC_TRANSITIVE) >>
         qexists_tac`bs2` >> simp[] >>
@@ -3450,9 +3490,9 @@ fun tac18 t =
         simp[Abbr`bs2`,bc_state_component_equality] >>
         simp[SUM_APPEND,FILTER_APPEND,TAKE_APPEND1,TAKE_APPEND2] ) >>
       fs[Abbr`bs2`,Abbr`bss0`] >>
-      reverse conj_tac >- metis_tac[IS_PREFIX_TRANS,SUBMAP_TRANS] >>
+      reverse conj_tac >- metis_tac[IS_PREFIX_TRANS,SUBMAP_TRANS,gvrel_trans] >>
       match_mp_tac Cenv_bs_imp_incsz_irr >>
-      qexists_tac`bs with <| refs := rf'; clock := ck'; code := bce|>` >>
+      qexists_tac`bs with <| refs := rf'; clock := ck'; code := bce; globals := gvv|>` >>
       simp[bc_state_component_equality] >>
       match_mp_tac Cenv_bs_pops >>
       qexists_tac`[br;bv]` >> simp[] >>
@@ -3515,9 +3555,9 @@ fun tac18 t =
         fs[Cenv_bs_def,s_refs_def,good_rd_def,FEVERY_DEF,SUBMAP_DEF,DRESTRICT_DEF,UNCURRY]) >>
       simp[code_for_return_def] >>
       simp_tac(srw_ss()++DNF_ss)[] >>
-      map_every qx_gen_tac[`br`,`rf'`,`rd''`,`ck'`] >>
+      map_every qx_gen_tac[`br`,`rf'`,`rd''`,`ck'`,`gvv`] >>
       strip_tac >>
-      map_every qexists_tac[`br`,`rf'`,`rd''`,`ck'`] >>
+      map_every qexists_tac[`br`,`rf'`,`rd''`,`ck'`,`gvv`] >>
       conj_tac >- (
         match_mp_tac(SIMP_RULE std_ss [transitive_def] RTC_TRANSITIVE) >>
         qmatch_assum_abbrev_tac`bc_next^* bs bs2` >>
@@ -3528,7 +3568,7 @@ fun tac18 t =
         fs[Abbr`bs4`] >>
         simp[Abbr`bs2`,Abbr`bss0`] ) >>
       fs[Abbr`bss0`] >>
-      metis_tac[IS_PREFIX_TRANS,SUBMAP_TRANS]) >>
+      metis_tac[IS_PREFIX_TRANS,SUBMAP_TRANS,gvrel_trans]) >>
     rpt gen_tac >>
     Q.PAT_ABBREV_TAC`cs2 = compiler_result_out_fupd (K (Stack X::Y)) B` >>
     qspecl_then[`t`,`cs2`](Q.X_CHOOSE_THEN`cp`strip_assume_tac)pushret_append_out >> pop_assum kall_tac >>
@@ -3591,9 +3631,9 @@ fun tac18 t =
       qexists_tac`args`>>simp[] ) >>
     simp[code_for_return_def] >>
     simp_tac(srw_ss()++DNF_ss)[] >>
-    map_every qx_gen_tac[`br`,`rf'`,`rd''`,`ck'`] >>
+    map_every qx_gen_tac[`br`,`rf'`,`rd''`,`ck'`,`gvv`] >>
     strip_tac >>
-    map_every qexists_tac[`br`,`rf'`,`rd''`,`ck'`] >>
+    map_every qexists_tac[`br`,`rf'`,`rd''`,`ck'`,`gvv`] >>
     conj_tac >- (
       match_mp_tac(SIMP_RULE std_ss [transitive_def] RTC_TRANSITIVE) >>
       qmatch_assum_abbrev_tac`bc_next^* bs bs2` >>
@@ -3606,7 +3646,8 @@ fun tac18 t =
       fs[Abbr`bs4`] >>
       simp[Abbr`bs2`,Abbr`bss0`] ) >>
     fs[Abbr`bss0`,Abbr`bs2`] >>
-    metis_tac[IS_PREFIX_TRANS,SUBMAP_TRANS]) >>
+    metis_tac[IS_PREFIX_TRANS,SUBMAP_TRANS,gvrel_trans]) >>
+
   strip_tac >- (
     simp[compile_def] >>
     rpt gen_tac >> strip_tac >>
@@ -5836,18 +5877,18 @@ fun tac18 t =
 
   strip_tac >- (
     rpt gen_tac >> strip_tac >>
-    simp[compile_def,pushret_def] >>
+    simp[compile_def,pushret_def,FOLDL_emit_append_out] >>
     rpt gen_tac >> strip_tac >>
-    qspecl_then[`cmnv`,`cenv`,`TCNonTail`,`sz`,`cs`,`exp`]strip_assume_tac (CONJUNCT1 compile_append_out) >>
+    qspecl_then[`cenv`,`TCNonTail`,`sz`,`cs`,`exp`]strip_assume_tac (CONJUNCT1 compile_append_out) >>
     simp[Once SWAP_REVERSE] >>
     simp[Once SWAP_REVERSE] >>
-    reverse(Cases_on`∃bc10. code = REVERSE bc ++ (prim1_to_bc uop)::bc10`) >- (
-      rw[] >> fs[] >> rfs[] >>
-      Cases_on`t`>>fs[pushret_def,Once SWAP_REVERSE]) >>
+    reverse(Cases_on`∃bc10. code = REVERSE bc ++ prim1_to_bc uop ++ bc10`) >- (
+      rw[] >> fs[FOLDL_emit_append_out] >> rfs[] >>
+      TRY(Cases_on`t`)>>fs[pushret_def,Once SWAP_REVERSE]) >>
     fs[] >>
-    reverse(Cases_on`bs.code = bc0 ++ REVERSE bc ++ [prim1_to_bc uop] ++ bc10 ++ bc1`) >- (
+    reverse(Cases_on`bs.code = bc0 ++ REVERSE bc ++ prim1_to_bc uop ++ bc10 ++ bc1`) >- (
       fs[]) >>
-    first_x_assum(qspecl_then[`rd`,`cmnv`,`cs`,`cenv`,`sz`,`csz`,`bs`,`bce`,`bcr`,`bc0`,`REVERSE bc`]mp_tac) >>
+    first_x_assum(qspecl_then[`rd`,`cs`,`cenv`,`sz`,`csz`,`bs`,`bce`,`bcr`,`bc0`,`REVERSE bc`]mp_tac) >>
     simp[Once SWAP_REVERSE] >>
     disch_then(assume_tac o CONJUNCT1) >>
     Cases_on`res`>>fs[] >- (
@@ -5860,16 +5901,20 @@ fun tac18 t =
         map_every qx_gen_tac[`rf`,`rd'`,`ck`,`bv`] >>
         strip_tac >>
         qmatch_assum_abbrev_tac`bc_next^* bs bs1` >>
-        qspecl_then[`rd'`,`uop`,`count'`,`s'`,`v`,`s''`,`a`,`bs1`,`bc0 ++ REVERSE bc`,`bc10++bc1`,`bce`,`bs.stack`,`bv`]
-          mp_tac prim1_to_bc_thm >>
+        qspecl_then[`rd'`,`uop`,`count'`,`(s',g)`,`v`,`(s'',g')`,`a`,`bs1`,`bc0 ++ REVERSE bc`,`bc10++bc1`,`bce`,`bs.stack`,`bv`]
+          mp_tac (INST_TYPE[alpha|->``:Cv``]prim1_to_bc_thm) >>
         simp[Abbr`bs1`] >>
         discharge_hyps >- fs[Cenv_bs_def] >>
-        disch_then(qx_choosel_then[`bvr`,`rfr`,`smr`]strip_assume_tac) >>
+        disch_then(qx_choosel_then[`bvr`,`rfr`,`gv`,`smr`]strip_assume_tac) >>
         map_every qexists_tac[`rfr`,`rd' with sm := smr`,`ck`,`bvr`] >>
         simp[] >>
         qmatch_assum_abbrev_tac`bc_next^* bs bs1` >>
-        qmatch_assum_abbrev_tac`bc_next bs1 bs2` >>
-        conj_tac >- metis_tac[RTC_TRANSITIVE,transitive_def,RTC_SUBSET] >>
+        qmatch_assum_abbrev_tac`bc_next^* bs1 bs2` >>
+
+        conj_tac >- (
+          qmatch_abbrev_tac`bc_next^* bs bs2'` >>
+          `bs2' = bs2`
+          metis_tac[RTC_TRANSITIVE,transitive_def,RTC_SUBSET] >>
         reverse conj_tac >- metis_tac[SUBMAP_TRANS,IS_PREFIX_TRANS] >>
         match_mp_tac Cenv_bs_imp_incsz_irr >>
         qexists_tac`bs with <| code := bce; refs := rfr; clock := ck|>`>>
